Prove the simple example in theory

src/ExampleSimple.v
@@ -1,12 +1,21 @@
 From sflib Require Import sflib.
 From Paco Require Import paco.
-
-Require Export Coq.Strings.String.
-From Coq Require Import Program.
-
-From Fairness Require Export ITreeLib WFLib FairBeh NatStructs Mod.
+Require Import Coq.Classes.RelationClasses Lia Program.
+From Fairness Require Export ITreeLib WFLib FairBeh NatStructs Mod pind.
 
 Set Implicit Arguments.
+
+(* TODO: move it to ITreeLib *)
+Lemma unfold_iter_eq A E B
+  : forall (f : A -> itree E (A + B)) (x : A),
+    ITree.iter f x = lr <- f x;; match lr with
+                                 | inl l => Tau (ITree.iter f l)
+                                 | inr r0 => Ret r0
+                                 end.
+Proof.
+  i. eapply bisim_is_eq. eapply unfold_iter.
+Qed.
+
 
 Section MOD.
   Definition example_fun:
@@ -52,19 +61,205 @@ Section MOD.
   .
 End MOD.
 
-From Fairness Require Import ModSim PCM.
+From Fairness Require Import IProp IPM Weakest.
+From Fairness Require Import ModSim PCM MonotonePCM ThreadsRA.
 
 Section SIM.
-  Context `{M: URA.t}.
+  Context `{Σ: GRA.t}.
+  Context `{MONORA: @GRA.inG monoRA Σ}.
+  Context `{THSRA: @GRA.inG ths_RA Σ}.
+  Context `{EXCL: @GRA.inG (Excl.t unit) Σ}.
 
-  Let I:
-    shared unit (bool * bool) void void nat_wf nat_wf -> M -> Prop :=
-        fun '(ths, im_src, im_tgt, st_src, st_tgt) w => True.
+  Variant W: Type :=
+    | W_bot
+    | W_own (th: thread_id) (i: nat)
+    | W_top
+  .
+
+  Variant W_le: W -> W -> Prop :=
+    | W_le_bot
+        w
+      :
+      W_le W_bot w
+    | W_le_th
+        th i0 i1
+        (LE: i0 <= i1)
+      :
+      W_le (W_own th i1) (W_own th i0)
+    | W_le_top
+        w
+      :
+      W_le w W_top
+  .
+
+  Program Instance W_le_PreOrder: PreOrder W_le.
+  Next Obligation.
+  Proof.
+    ii. destruct x; econs. lia.
+  Qed.
+  Next Obligation.
+  Proof.
+    ii. inv H; inv H0; try econs; eauto. lia.
+  Qed.
+
+  Let I: TIdSet.t -> (@imap void nat_wf) -> (@imap (sum_tid void) nat_wf) -> unit -> (bool * bool) -> iProp :=
+        fun ths im_src im_tgt st_src '(l, f) =>
+          (∃ w,
+              (own_threads ths)
+                **
+                (monoBlack 0 W_le_PreOrder w)
+                **
+                (match w with
+                 | W_bot => ⌜l = false⌝ ** (OwnM (Excl.just tt: @URA.car (Excl.t unit)))
+                 | W_own th i => ⌜l = true /\ im_tgt (inl th) = i⌝ ** own_thread th
+                 | W_top => ⌜l = true /\ f = true⌝ ** (OwnM (Excl.just tt: @URA.car (Excl.t unit)))
+                 end))%I.
+
+  Let srcE := ((@eventE void +' cE) +' sE unit).
+  Let tgtE := ((@eventE void +' cE) +' sE (bool * bool)).
+
+  Definition itop10 { T0 T1 T2 T3 T4 T5 T6 T7 T8 T9} (x0: T0) (x1: T1 x0) (x2: T2 x0 x1) (x3: T3 x0 x1 x2) (x4: T4 x0 x1 x2 x3) (x5: T5 x0 x1 x2 x3 x4) (x6: T6 x0 x1 x2 x3 x4 x5) (x7: T7 x0 x1 x2 x3 x4 x5 x6) (x8: T8 x0 x1 x2 x3 x4 x5 x6 x7) (x9: T9 x0 x1 x2 x3 x4 x5 x6 x7 x8): iProp := True%I.
+
+  Definition isim_gen tid r g R_src R_tgt Q (itr_src: itree srcE R_src) (itr_tgt: itree tgtE R_tgt): iProp :=
+    ∀ ths im_src im_tgt0 st_src st_tgt im_tgt1,
+      I ths im_src im_tgt0 st_src st_tgt
+        -*
+        ⌜fair_update im_tgt0 im_tgt1 (sum_fmap_l (tids_fmap tid ths))⌝
+        -*
+        isim tid I r g Q itr_src itr_tgt ths im_src im_tgt1 st_src st_tgt.
 
   Lemma sim: ModSim.mod_sim example_mod_spec example_mod.
   Proof.
-    eapply (@ModSim.mk _ _ nat_wf nat_wf _ _ M). instantiate (1:=I).
-    { ii. admit. }
-    i. ss. ii.
+    eapply (@ModSim.mk _ _ nat_wf nat_wf _ _ Σ).
+    { instantiate (1:=liftI I). admit. }
+    i. ss.
+    cut (forall tid, own_thread tid ⊢ @isim_gen tid itop10 itop10 _ _ (fun r_src r_tgt ths im_src im_tgt st_src st_tgt => I ths im_src im_tgt st_src st_tgt ** ⌜r_src = r_tgt⌝) example_fun_spec example_fun).
+    { admit. }
+
+    unfold isim_gen. i. iIntros "TID".
+    iIntros (ths im_src im_tgt0 st_src st_tgt im_tgt1) "INV %H".
+    unfold I. des_ifs.
+    iDestruct "INV" as (w) "[[THS MONO] INV]".
+    destruct w.
+
+    3:{
+      iPoseProof (black_persistent_white with "MONO") as "#WHITE".
+      iDestruct "INV" as "[% OWN]". des. subst.
+      unfold example_fun_spec, example_fun.
+      iApply isim_getR.
+      ired. rewrite unfold_iter_eq. ired.
+      iApply isim_getR. ired.
+      iApply isim_sync.
+      iSplitL.
+      { iExists W_top. iFrame. iPureIntro. auto. }
+      iIntros (ths1 im_src1 im_tgt2 st_src1 st_tgt1 im_tgt3) "INV".
+      iIntros. iApply isim_ret. iSplitL; auto. des_ifs.
+      iDestruct "INV" as (w) "[[THS MONO] INV]".
+      iPoseProof (black_white_compare with "WHITE MONO") as "%".
+      inv H1. iExists W_top. iFrame.
+    }
+
+    1:{
+      iPoseProof (black_persistent_white with "MONO") as "#WHITE".
+      iDestruct "INV" as "[% OWN]". subst.
+      unfold example_fun_spec, example_fun.
+      iApply isim_getR.
+      iApply isim_putR.
+      iAssert (⌜W_le W_bot (W_own tid (im_tgt1 (inl tid)))⌝)%I as "LE".
+      { iPureIntro. econs. }
+      iPoseProof (black_updatable with "MONO LE") as "> MONO".
+      iClear "WHITE".
+      iPoseProof (black_persistent_white with "MONO") as "#WHITE".
+      iApply isim_sync. iSplitR "OWN".
+      { iExists (W_own tid _). iFrame. auto. }
+      iIntros (ths1 im_src1 im_tgt2 st_src1 st_tgt1 im_tgt3) "INV %".
+      des_ifs. iDestruct "INV" as (w) "[[THS MONO] INV]".
+      iPoseProof (black_white_compare with "WHITE MONO") as "%".
+      inv H1.
+      2:{ iDestruct "INV" as "[% INV]".
+          iCombine "OWN INV" as "OWN". iOwnWf "OWN". ur in H2. ss.
+      }
+      iApply isim_getR. iApply isim_putR.
+      iClear "LE".
+      iAssert (⌜W_le (W_own tid i0) W_top⌝)%I as "LE".
+      { iPureIntro. econs. }
+      iPoseProof (black_updatable with "MONO LE") as "> MONO".
+      iApply isim_ret. iSplitL; auto.
+      iExists W_top. iFrame. iDestruct "INV" as "[% INV]". des. subst. auto.
+    }
+
+    {
+      iPoseProof (black_persistent_white with "MONO") as "#WHITE".
+      iDestruct "INV" as "[% OWN]". des. subst.
+      unfold example_fun_spec, example_fun.
+      remember (im_tgt0 (inl th)).
+
+      iApply isim_getR.
+
+      iStopProof.
+      revert ths im_src st_src im_tgt0 im_tgt1 b0 th Heqt H.
+      induction (Nat.lt_wf_0 t). clear H. rename H0 into IH.
+      i. subst.
+      iIntros "[WHITE [TID [THS [MONO OWN]]]]".
+
+      iPoseProof (thread_disjoint with "TID OWN") as "%".
+      iAssert (⌜W_le (W_own th (im_tgt0 (inl th))) (W_own th (im_tgt1 (inl th)))⌝)%I as "LE".
+      { iPureIntro. econs.
+        specialize (H (inl th)).
+        unfold sum_fmap_l, tids_fmap in H. des_ifs.
+        { ss. lia. }
+        { lia. }
+      }
+      iPoseProof (black_updatable with "MONO LE") as "> MONO".
+      iClear "WHITE".
+      iPoseProof (black_persistent_white with "MONO") as "#WHITE".
+
+      rewrite unfold_iter_eq. ired.
+      iApply isim_getR. destruct b0.
+      { ired.
+        iApply isim_sync.
+        iSplitL.
+        { iExists (W_own _ _). iFrame. iPureIntro. auto. }
+        iIntros (ths1 im_src1 im_tgt2 st_src1 st_tgt1 im_tgt3) "INV".
+        iIntros. iApply isim_ret. iSplitL; auto. des_ifs.
+        iDestruct "INV" as (w) "[[THS MONO] INV]".
+        iPoseProof (black_white_compare with "WHITE MONO") as "%".
+        inv H2.
+        admit. admit.
+      }
+
+      { ired.
+        iApply isim_yieldR.
+        { iSplitR "TID".
+          { iExists (W_own _ _). iFrame. iPureIntro. auto. }
+          iIntros (ths1 im_src1 im_tgt2 st_src1 st_tgt1 im_tgt3) "INV".
+          iIntros. iApply isim_tauR.
+          des_ifs.
+          iDestruct "INV" as (w) "[[THS MONO] INV]".
+          iPoseProof (black_white_compare with "WHITE MONO") as "%".
+          inv H2.
+          2:{ iDestruct "INV" as "[% INV]". des. subst.
+              rewrite unfold_iter_eq. ired.
+              iApply isim_getR. ired.
+              iApply isim_sync. iSplitL.
+              { iExists W_top. iFrame. auto. }
+              { admit. }
+          }
+          { iDestruct "INV" as "[% INV]". des. subst.
+            iApply IH.
+            3:{ eauto. }
+            2:{ reflexivity. }
+            { instantiate (1:=th).
+              cut (im_tgt1 (inl th) < im_tgt0 (inl th)).
+              { lia. }
+              specialize (H (inl th)). unfold sum_fmap_l, tids_fmap in H.
+              des_ifs. admit.
+            }
+            iClear "WHITE".
+            iPoseProof (black_persistent_white with "MONO") as "#WHITE".
+            iFrame. auto.
+          }
+        }
+      }
   Admitted.
 End SIM.
