src/ThreadsRA.v
@@ -1,0 +1,37 @@
+From sflib Require Import sflib.
+Require Import Coq.Classes.RelationClasses.
+From Fairness Require Import Axioms NatStructs.
+From Fairness Require Import PCM World IProp IPM.
+From Fairness Require Import Mod.
+Require Import String Lia Program.
+
+Set Implicit Arguments.
+
+Section THREADS_RA_DEF.
+  Definition ths_RA: URA.t. Admitted.
+
+  Definition ths_RA_set (ths: TIdSet.t): ths_RA.(URA.car). Admitted.
+
+  Definition ths_RA_th (th: thread_id): ths_RA.(URA.car). Admitted.
+
+  Context `{@GRA.inG ths_RA Σ}.
+
+  Definition own_threads (ths: TIdSet.t): iProp := OwnM (ths_RA_set ths).
+
+  Definition own_thread (th: thread_id): iProp := OwnM (ths_RA_th th).
+
+  Lemma thread_disjoint th0 th1
+    :
+    (own_thread th0) -∗ (own_thread th1) -∗ ⌜th0 <> th1⌝.
+  Admitted.
+
+  Lemma threads_alloc tid ths0 ths1
+    :
+    own_threads ths0 -∗ ⌜TIdSet.add_new tid ths0 ths1⌝ -∗ (own_threads ths1 ** own_thread tid).
+  Admitted.
+
+  Lemma threads_dealloc tid ths0
+    :
+    own_threads ths0 -∗ own_thread tid -∗ ∃ ths1, ⌜NatMap.remove tid ths0 = ths1⌝ ** own_threads ths1.
+  Admitted.
+End THREADS_RA_DEF.
